txn-data-consistency/Prot_2PC_2PL.thy
@@ -15,11 +15,11 @@ datatype status_tm = tm_init | tm_prepared | tm_committed | tm_aborted
 record tm_state =
   tm_status :: status_tm
   tm_sn :: nat
-  (*tm_view :: view -- We used the global_view (seeing everything)*)
+  (*tm_view :: view -- We used the full_view (seeing everything)*)
 
 \<comment>\<open>Key Manager (KM)\<close>
 record 'v km_state =
-  km_vl :: "'v version list"
+  km_vl :: "'v v_list"
   km_key_fp :: "txid0 \<Rightarrow> 'v key_fp"
   km_status :: "txid0 \<Rightarrow> status_km"
 
@@ -31,22 +31,29 @@ record 'v global_state =
 
 subsubsection \<open>Events\<close>
 
-datatype 'v km_ev = Write2 txid0 'v | Read2 txid0 'v | Prepare txid0 | RLock txid0 | WLock txid0 |
-                    NoLock txid0 | NOK txid0 | Commit txid0 | Abort txid0
-datatype tm_ev = User_Commit | TM_Commit | TM_Abort | TM_ReadyC | TM_ReadyA | TM_Skip
-datatype 'v ev = KM_ev key "'v km_ev" | TM_ev cl_id tm_ev
+datatype 'v ev = Write2 key txid0 'v | Read2 key txid0 'v | Prepare key txid0 | RLock key txid0 |
+  WLock key txid0 | NoLock key txid0 | NOK key txid0 | Commit key txid0 | Abort key txid0 |
+  User_Commit cl_id | TM_Commit cl_id sqn view "'v fingerpr"| TM_Abort cl_id | TM_ReadyC cl_id |
+  TM_ReadyA cl_id | Skip2
 
-definition other_instances_unchanged where
-  "other_instances_unchanged t k kmss kmss' \<equiv> (\<forall>t'. t' \<noteq> t \<longrightarrow>
+definition km_t'_unchanged where
+  "km_t'_unchanged t k kmss kmss' \<equiv> (\<forall>t'. t' \<noteq> t \<longrightarrow>
      km_key_fp (kmss' k) t' = km_key_fp (kmss k) t' \<and>
      km_status (kmss' k) t' = km_status (kmss k) t')"
 
-definition other_kms_unchanged where
-  "other_kms_unchanged k kmss kmss' \<equiv> (\<forall>k'. k' \<noteq> k \<longrightarrow> kmss' k' = kmss k')"
+definition other_insts_unchanged where
+  "other_insts_unchanged k kmss kmss' \<equiv> (\<forall>k'. k' \<noteq> k \<longrightarrow> kmss' k' = kmss k')"
 
-abbreviation tm_other_kms_unchanged where
-  "tm_other_kms_unchanged k s s' t \<equiv> tm s' = tm s \<and>
-    other_kms_unchanged k (kms s) (kms s') \<and> other_instances_unchanged t k (kms s) (kms s')"
+definition tm_km_k'_t'_unchanged where
+  "tm_km_k'_t'_unchanged k s s' t \<equiv> tm s' = tm s \<and>
+    other_insts_unchanged k (kms s) (kms s') \<and> km_t'_unchanged t k (kms s) (kms s')"
+
+definition km_tm_cl'_unchanged where
+  "km_tm_cl'_unchanged cl s s' \<equiv> kms s' = kms s \<and> other_insts_unchanged cl (tm s) (tm s')"
+
+lemmas km_unchanged_defs = tm_km_k'_t'_unchanged_def other_insts_unchanged_def km_t'_unchanged_def
+lemmas tm_unchanged_defs = km_tm_cl'_unchanged_def other_insts_unchanged_def
+lemmas unchanged_defs = km_unchanged_defs km_tm_cl'_unchanged_def
 
 abbreviation km_status_trans where
   "km_status_trans s k s' t from_stat to_stat \<equiv>
@@ -54,7 +61,7 @@ abbreviation km_status_trans where
     \<and> km_vl (kms s' k) = km_vl (kms s k)
     \<and> km_key_fp (kms s' k) = km_key_fp (kms s k)
     \<and> km_status (kms s' k) t = to_stat
-    \<and> tm_other_kms_unchanged k s s' t"
+    \<and> tm_km_k'_t'_unchanged k s s' t"
 
 fun get_cl_txn :: "txid0 \<Rightarrow> cl_id" where
   "get_cl_txn (Tn_cl sn cl) = cl"
@@ -67,27 +74,25 @@ fun get_txn_cl :: "cl_id \<Rightarrow> 'v global_state \<Rightarrow> txid0" wher
 
 \<comment>\<open> Might be a good idea to check if Tn_cl sn cl = t. Not used yet.\<close>
 definition tid_match :: "'v global_state \<Rightarrow> txid0 \<Rightarrow> bool" where
-  "tid_match s t \<equiv> tm_sn (tm s (get_cl_txn t)) = get_sn_txn t "
-
-definition global_view :: "'v v_list \<Rightarrow> key_view" where
-  "global_view vl \<equiv> {0.. (length vl)}"
-
+  "tid_match s t \<equiv> tm_sn (tm s (get_cl_txn t)) = get_sn_txn t"
 
 definition write2 where
   "write2 s k v s' t \<equiv>
     km_status (kms s k) t = working
+    \<and> tid_match s t
     \<and> km_key_fp (kms s' k) t = update_key_fp (km_key_fp (kms s k) t) W v
     \<and> km_status (kms s' k) t = working
     \<and> km_vl (kms s' k) = km_vl (kms s k)
-    \<and> tm_other_kms_unchanged k s s' t"
+    \<and> tm_km_k'_t'_unchanged k s s' t"
 
 definition read2 where
   "read2 s k v s' t  \<equiv>
     km_status (kms s k) t = working
+    \<and> tid_match s t
     \<and> km_key_fp (kms s' k) t = update_key_fp (km_key_fp (kms s k) t) R v
     \<and> km_status (kms s' k) t = working
     \<and> km_vl (kms s' k) = km_vl (kms s k)
-    \<and> tm_other_kms_unchanged k s s' t"
+    \<and> tm_km_k'_t'_unchanged k s s' t"
 
 definition prepare where
   "prepare s k s' t \<equiv>
@@ -114,6 +119,7 @@ definition acquire_no_lock where \<comment>\<open>No Lock needed\<close>
     tm_status (tm s (get_cl_txn t)) = tm_prepared
     \<and> km_key_fp (kms s k) t W = None
     \<and> km_key_fp (kms s k) t R = None
+    \<and> (\<forall>t'. km_status (kms s k) t' \<in> {working, prepared, read_lock, write_lock, no_lock, notokay})
     \<and> km_status_trans s k s' t prepared no_lock"
 
 definition nok where \<comment>\<open>Lock not available\<close>
@@ -130,10 +136,10 @@ definition commit where
     km_status (kms s k) t \<in> {read_lock, write_lock, no_lock}
     \<and> tm_status (tm s (get_cl_txn t)) = tm_committed
     \<and> km_vl (kms s' k) =
-        update_kv_key t (km_key_fp (kms s k) t) (global_view (km_vl (kms s k))) (km_vl (kms s k))
+        update_kv_key t (km_key_fp (kms s k) t) (full_view (km_vl (kms s k))) (km_vl (kms s k))
     \<and> km_key_fp (kms s' k) t = Map.empty
     \<and> km_status (kms s' k) t = committed
-    \<and> tm_other_kms_unchanged k s s' t"
+    \<and> tm_km_k'_t'_unchanged k s s' t"
 
 definition abort where \<comment>\<open>Locks released (aborted)\<close>
   "abort s k s' t \<equiv>
@@ -142,22 +148,25 @@ definition abort where \<comment>\<open>Locks released (aborted)\<close>
     \<and> km_vl (kms s' k) = km_vl (kms s k)
     \<and> km_key_fp (kms s' k) t = Map.empty
     \<and> km_status (kms s' k) t = aborted
-    \<and> tm_other_kms_unchanged k s s' t"
+    \<and> tm_km_k'_t'_unchanged k s s' t"
 
 definition user_commit where
   "user_commit s s' cl \<equiv>
     tm_status (tm s cl) = tm_init
     \<and> tm_status (tm s' cl) = tm_prepared
     \<and> tm_sn (tm s' cl) = tm_sn (tm s cl)
-    \<and> kms s' = kms s"
+    \<and> km_tm_cl'_unchanged cl s s'"
 
 definition tm_commit where
-  "tm_commit s s' cl \<equiv>
+  "tm_commit s s' cl sn u F \<equiv>
     tm_status (tm s cl) = tm_prepared
     \<and> (\<forall>k. km_status (kms s k) (get_txn_cl cl s) \<in> {read_lock, write_lock, no_lock})
     \<and> tm_status (tm s' cl) = tm_committed
     \<and> tm_sn (tm s' cl) = tm_sn (tm s cl)
-    \<and> kms s' = kms s"
+    \<and> km_tm_cl'_unchanged cl s s'
+    \<and> sn = tm_sn (tm s cl)
+    \<and> u = (\<lambda>k. full_view (km_vl (kms s k)))
+    \<and> F = (\<lambda>k. km_key_fp (kms s k) (get_txn_cl cl s))"
 
 definition tm_abort where
   "tm_abort s s' cl \<equiv>
@@ -166,7 +175,7 @@ definition tm_abort where
      \<and> (\<forall>k. km_status (kms s k) (get_txn_cl cl s) \<in> {read_lock, write_lock, no_lock, notokay}))
     \<and> tm_status (tm s' cl) = tm_aborted
     \<and> tm_sn (tm s' cl) = tm_sn (tm s cl)
-    \<and> kms s' = kms s"
+    \<and> km_tm_cl'_unchanged cl s s'"
 
 definition tm_ready_c where
   "tm_ready_c s s' cl \<equiv>
@@ -174,7 +183,7 @@ definition tm_ready_c where
     \<and> (\<forall>k. km_status (kms s k) (get_txn_cl cl s) = committed)
     \<and> tm_status (tm s' cl) = tm_init
     \<and> tm_sn (tm s' cl) = Suc (tm_sn (tm s cl))
-    \<and> kms s' = kms s"
+    \<and> km_tm_cl'_unchanged cl s s'"
 
 definition tm_ready_a where
   "tm_ready_a s s' cl \<equiv>
@@ -182,7 +191,7 @@ definition tm_ready_a where
     \<and> (\<forall>k. km_status (kms s k) (get_txn_cl cl s) = aborted)
     \<and> tm_status (tm s' cl) = tm_init
     \<and> tm_sn (tm s' cl) = Suc (tm_sn (tm s cl))
-    \<and> kms s' = kms s"
+    \<and> km_tm_cl'_unchanged cl s s'"
 
 text\<open>The Event System\<close>
 definition gs_init :: "'v global_state" where
@@ -194,21 +203,21 @@ definition gs_init :: "'v global_state" where
   \<rparr>"
 
 fun gs_trans :: "'v global_state \<Rightarrow> 'v ev \<Rightarrow> 'v global_state \<Rightarrow> bool" where
-  "gs_trans s (KM_ev k (Write2 t v)) s' \<longleftrightarrow> write2 s k v s' t" |
-  "gs_trans s (KM_ev k (Read2 t v))  s' \<longleftrightarrow> read2 s k v s' t" |
-  "gs_trans s (KM_ev k (Prepare t))  s' \<longleftrightarrow> prepare s k s' t" |
-  "gs_trans s (KM_ev k (RLock t))    s' \<longleftrightarrow> acquire_rd_lock s k s' t" |
-  "gs_trans s (KM_ev k (WLock t))    s' \<longleftrightarrow> acquire_wr_lock s k s' t" |
-  "gs_trans s (KM_ev k (NoLock t))   s' \<longleftrightarrow> acquire_no_lock s k s' t" |
-  "gs_trans s (KM_ev k (NOK t))      s' \<longleftrightarrow> nok s k s' t" |
-  "gs_trans s (KM_ev k (Commit t))   s' \<longleftrightarrow> commit s k s' t" |
-  "gs_trans s (KM_ev k (Abort t))    s' \<longleftrightarrow> abort s k s' t" |
-  "gs_trans s (TM_ev cl User_Commit) s' \<longleftrightarrow> user_commit s s' cl" |
-  "gs_trans s (TM_ev cl TM_Commit)   s' \<longleftrightarrow> tm_commit s s' cl" |
-  "gs_trans s (TM_ev cl TM_Abort)    s' \<longleftrightarrow> tm_abort s s' cl" |
-  "gs_trans s (TM_ev cl TM_ReadyC)   s' \<longleftrightarrow> tm_ready_c s s' cl" |
-  "gs_trans s (TM_ev cl TM_ReadyA)   s' \<longleftrightarrow> tm_ready_a s s' cl" |
-  "gs_trans s (TM_ev cl TM_Skip)     s' \<longleftrightarrow> s' = s"
+  "gs_trans s (Write2 k t v)        s' \<longleftrightarrow> write2 s k v s' t" |
+  "gs_trans s (Read2 k t v)         s' \<longleftrightarrow> read2 s k v s' t" |
+  "gs_trans s (Prepare k t)         s' \<longleftrightarrow> prepare s k s' t" |
+  "gs_trans s (RLock k t)           s' \<longleftrightarrow> acquire_rd_lock s k s' t" |
+  "gs_trans s (WLock k t)           s' \<longleftrightarrow> acquire_wr_lock s k s' t" |
+  "gs_trans s (NoLock k t)          s' \<longleftrightarrow> acquire_no_lock s k s' t" |
+  "gs_trans s (NOK k t)             s' \<longleftrightarrow> nok s k s' t" |
+  "gs_trans s (Commit k t)          s' \<longleftrightarrow> commit s k s' t" |
+  "gs_trans s (Abort k t)           s' \<longleftrightarrow> abort s k s' t" |
+  "gs_trans s (User_Commit cl)      s' \<longleftrightarrow> user_commit s s' cl" |
+  "gs_trans s (TM_Commit cl sn u F) s' \<longleftrightarrow> tm_commit s s' cl sn u F" |
+  "gs_trans s (TM_Abort cl)         s' \<longleftrightarrow> tm_abort s s' cl" |
+  "gs_trans s (TM_ReadyC cl)        s' \<longleftrightarrow> tm_ready_c s s' cl" |
+  "gs_trans s (TM_ReadyA cl)        s' \<longleftrightarrow> tm_ready_a s s' cl" |
+  "gs_trans s Skip2                 s' \<longleftrightarrow> s' = s"
 
 definition tps :: "('v ev, 'v global_state) ES" where
   "tps \<equiv> \<lparr>
@@ -223,6 +232,652 @@ lemmas tps_trans_defs = write2_def read2_def prepare_def acquire_rd_lock_def acq
 lemmas tps_defs = tps_def gs_init_def
 
 lemma tps_trans [simp]: "trans tps = gs_trans" by (simp add: tps_def)
+
+subsection \<open>Invariants\<close>
+
+text\<open>Auxiliary invariants about TM states\<close>
+definition TCInit where
+  "TCInit s \<longleftrightarrow> (\<forall>cl. (tm_status (tm s cl) = tm_init
+    \<longrightarrow> (\<forall>k. tid_match s (get_txn_cl cl s) \<and> km_status (kms s k) (get_txn_cl cl s) = working) \<or>
+        (\<forall>k. km_status (kms s k) (get_txn_cl cl s) = committed) \<or>
+        (\<forall>k. km_status (kms s k) (get_txn_cl cl s) = aborted)))"
+
+lemmas TCInitI = TCInit_def[THEN iffD2, rule_format]
+lemmas TCInitE[elim] = TCInit_def[THEN iffD1, elim_format, rule_format]
+
+lemma reach_tcinit [simp, dest]: "reach tps s \<Longrightarrow> TCInit s"
+proof(induction s rule: reach.induct)
+  case (reach_init s)
+  then show ?case
+  by (auto simp add: TCInit_def tps_defs tid_match_def)
+next
+  case (reach_trans s e s')
+  then show ?case 
+  proof (cases e)
+    case (Write2 x11 x12 x13)
+    then show ?thesis using reach_trans
+      apply (auto simp add: tps_trans_defs km_unchanged_defs tid_match_def TCInit_def) by fastforce
+  next
+    case (Read2 x21 x22 x23)
+    then show ?thesis using reach_trans
+      apply (auto simp add: tps_trans_defs km_unchanged_defs tid_match_def TCInit_def) by fastforce
+  next
+    case (Prepare x31 x32)
+    then show ?thesis using reach_trans
+      apply (auto simp add: tps_trans_defs km_unchanged_defs tid_match_def TCInit_def)
+      by (smt get_cl_txn.simps status_tm.distinct(1))
+  next
+    case (RLock x41 x42)
+    then show ?thesis using reach_trans
+      apply (auto simp add: tps_trans_defs km_unchanged_defs tid_match_def TCInit_def)
+      by (smt get_cl_txn.simps status_tm.distinct(1))
+  next
+    case (WLock x51 x52)
+    then show ?thesis using reach_trans
+      apply (auto simp add: tps_trans_defs km_unchanged_defs tid_match_def TCInit_def)
+      by (smt status_km.distinct(1) status_km.distinct(23) status_km.distinct(25))
+  next
+    case (NoLock x61 x62)
+    then show ?thesis using reach_trans
+      apply (auto simp add: tps_trans_defs km_unchanged_defs tid_match_def TCInit_def)
+      by (smt status_km.distinct(1) status_km.distinct(23) status_km.distinct(25))
+  next
+    case (NOK x71 x72)
+    then show ?thesis using reach_trans
+      apply (auto simp add: tps_trans_defs km_unchanged_defs tid_match_def TCInit_def)
+      by (smt status_km.distinct(1) status_km.distinct(23) status_km.distinct(25))+
+  next
+    case (Commit x81 x82)
+    then show ?thesis using reach_trans
+      apply (auto simp add: tps_trans_defs km_unchanged_defs tid_match_def TCInit_def)
+      by fastforce+
+  next
+    case (Abort x91 x92)
+    then show ?thesis using reach_trans
+      apply (auto simp add: tps_trans_defs km_unchanged_defs tid_match_def TCInit_def)
+      by fastforce+
+  next
+    case (User_Commit x10)
+    then show ?thesis using reach_trans
+      apply (auto simp add: tps_trans_defs tm_unchanged_defs tid_match_def TCInit_def)
+      by metis
+  next
+    case (TM_Commit x111 x112 x113 x114)
+    then show ?thesis using reach_trans
+      apply (auto simp add: tps_trans_defs tm_unchanged_defs tid_match_def TCInit_def)
+      by (metis status_tm.distinct(3))
+  next
+    case (TM_Abort x12a)
+    then show ?thesis using reach_trans
+      apply (auto simp add: tps_trans_defs tm_unchanged_defs tid_match_def TCInit_def)
+      by (metis status_tm.distinct(5))
+  next
+    case (TM_ReadyC x13a)
+    then show ?thesis using reach_trans
+      apply (auto simp add: tps_trans_defs tm_unchanged_defs tid_match_def TCInit_def) sorry
+  next
+    case (TM_ReadyA x14)
+    then show ?thesis using reach_trans
+      apply (auto simp add: tps_trans_defs tm_unchanged_defs tid_match_def TCInit_def) sorry
+  qed simp
+qed
+
+definition TCPrepared where
+  "TCPrepared s \<longleftrightarrow> (\<forall>cl. tm_status (tm s cl) = tm_prepared \<longrightarrow>
+    (\<forall>k. tid_match s (get_txn_cl cl s) \<and>
+      km_status (kms s k) (get_txn_cl cl s)
+      \<in> {working, prepared, read_lock, write_lock, no_lock, notokay}))"
+
+lemmas TCPreparedI = TCPrepared_def[THEN iffD2, rule_format]
+lemmas TCPreparedE[elim] = TCPrepared_def[THEN iffD1, elim_format, rule_format]
+
+lemma reach_tcprepared [simp, intro]: "reach tps s \<Longrightarrow> TCPrepared s"
+proof(induction s rule: reach.induct)
+  case (reach_init s)
+  then show ?case
+  by (auto simp add: TCPrepared_def tps_defs)
+next
+  case (reach_trans s e s')
+  then show ?case 
+  proof (cases e)
+    case (Write2 x11 x12 x13)
+    then show ?thesis using reach_trans
+      apply (auto simp add: tps_trans_defs km_unchanged_defs tid_match_def TCPrepared_def)
+      by smt
+  next
+    case (Read2 x21 x22 x23)
+    then show ?thesis using reach_trans
+      apply (auto simp add: tps_trans_defs km_unchanged_defs tid_match_def TCPrepared_def)
+      by smt
+  next      
+    case (Prepare x31 x32)
+    then show ?thesis using reach_trans
+      apply (auto simp add: tps_trans_defs km_unchanged_defs tid_match_def TCPrepared_def)
+      by smt
+  next
+    case (RLock x41 x42)
+    then show ?thesis using reach_trans
+      apply (auto simp add: tps_trans_defs km_unchanged_defs tid_match_def TCPrepared_def)
+      by smt
+  next
+    case (WLock x51 x52)
+    then show ?thesis using reach_trans
+      apply (auto simp add: tps_trans_defs km_unchanged_defs tid_match_def TCPrepared_def)
+      by smt
+  next
+    case (NoLock x61 x62)
+    then show ?thesis using reach_trans
+      apply (auto simp add: tps_trans_defs km_unchanged_defs tid_match_def TCPrepared_def)
+      by smt
+  next
+    case (NOK x71 x72)
+    then show ?thesis using reach_trans
+      apply (auto simp add: tps_trans_defs km_unchanged_defs tid_match_def TCPrepared_def)
+      by smt+
+  next
+    case (Commit x81 x82)
+    then show ?thesis using reach_trans
+      apply (auto simp add: tps_trans_defs km_unchanged_defs tid_match_def TCPrepared_def)
+      by (smt get_cl_txn.simps status_tm.distinct(7))+
+  next
+    case (Abort x91 x92)
+    then show ?thesis using reach_trans
+      apply (auto simp add: tps_trans_defs km_unchanged_defs tid_match_def TCPrepared_def)
+      by (smt get_cl_txn.simps status_tm.distinct(9))+
+  next
+    case (User_Commit x10)
+    then show ?thesis using reach_trans
+      apply (auto simp add: tps_trans_defs tm_unchanged_defs tid_match_def TCPrepared_def) sorry
+  next
+    case (TM_Commit x111 x112 x113 x114)
+    then show ?thesis using reach_trans
+      apply (auto simp add: tps_trans_defs tm_unchanged_defs tid_match_def TCPrepared_def)
+      by smt
+  next
+    case (TM_Abort x12a)
+    then show ?thesis using reach_trans
+      apply (auto simp add: tps_trans_defs tm_unchanged_defs tid_match_def TCPrepared_def)
+      by smt
+  next
+    case (TM_ReadyC x13a)
+    then show ?thesis using reach_trans
+      apply (auto simp add: tps_trans_defs tm_unchanged_defs tid_match_def TCPrepared_def)
+      by (smt status_tm.distinct(1))
+  next
+    case (TM_ReadyA x14)
+    then show ?thesis using reach_trans
+      apply (auto simp add: tps_trans_defs tm_unchanged_defs tid_match_def TCPrepared_def)
+      by (smt status_tm.distinct(1))
+  qed simp
+qed
+
+definition TCCommitted where
+  "TCCommitted s \<longleftrightarrow> (\<forall>cl. tm_status (tm s cl) = tm_committed \<longrightarrow> 
+    (\<forall>k. tid_match s (get_txn_cl cl s) \<and>
+     km_status (kms s k) (get_txn_cl cl s) \<in> {read_lock, write_lock, no_lock, committed}))"
+
+lemmas TCCommittedI = TCCommitted_def[THEN iffD2, rule_format]
+lemmas TCCommittedE[elim] = TCCommitted_def[THEN iffD1, elim_format, rule_format]
+
+lemma reach_tccommitted [simp, intro]: "reach tps s \<Longrightarrow> TCCommitted s"
+proof(induction s rule: reach.induct)
+  case (reach_init s)
+  then show ?case
+  by (auto simp add: TCCommitted_def tps_defs)
+next
+  case (reach_trans s e s')
+  then show ?case 
+  proof (cases e)
+    case (Write2 x11 x12 x13)
+    then show ?thesis using reach_trans
+      by (auto simp add: tps_trans_defs km_unchanged_defs tid_match_def TCCommitted_def, metis)
+  next
+    case (Read2 x21 x22 x23)
+    then show ?thesis using reach_trans
+      by (auto simp add: tps_trans_defs km_unchanged_defs tid_match_def TCCommitted_def, metis)
+  next
+    case (Prepare x31 x32)
+    then show ?thesis using reach_trans
+      apply (auto simp add: tps_trans_defs km_unchanged_defs tid_match_def TCCommitted_def)
+      by (metis get_cl_txn.simps status_tm.distinct(7))
+  next
+    case (RLock x41 x42)
+    then show ?thesis using reach_trans
+      by (auto simp add: tps_trans_defs km_unchanged_defs tid_match_def TCCommitted_def, smt)
+  next
+    case (WLock x51 x52)
+    then show ?thesis using reach_trans
+      by (auto simp add: tps_trans_defs km_unchanged_defs tid_match_def TCCommitted_def, smt)
+  next
+    case (NoLock x61 x62)
+    then show ?thesis using reach_trans
+      by (auto simp add: tps_trans_defs km_unchanged_defs tid_match_def TCCommitted_def, smt)
+  next
+    case (NOK x71 x72)
+    then show ?thesis using reach_trans
+      apply (auto simp add: tps_trans_defs km_unchanged_defs tid_match_def TCCommitted_def)
+      by (metis get_cl_txn.simps status_tm.distinct(7))+
+  next
+    case (Commit x81 x82)
+    then show ?thesis using reach_trans
+      by (auto simp add: tps_trans_defs km_unchanged_defs tid_match_def TCCommitted_def, metis+)
+  next
+    case (Abort x91 x92)
+    then show ?thesis using reach_trans
+      apply (auto simp add: tps_trans_defs km_unchanged_defs tid_match_def TCCommitted_def)
+      by (metis get_cl_txn.simps status_tm.distinct(11))+
+  next
+    case (User_Commit x10)
+    then show ?thesis using reach_trans
+      apply (auto simp add: tps_trans_defs tm_unchanged_defs tid_match_def TCCommitted_def)
+      by (metis status_tm.distinct(7))
+  next
+    case (TM_Commit x111 x112 x113 x114)
+    then show ?thesis using reach_trans
+      by (auto simp add: tps_trans_defs tm_unchanged_defs tid_match_def TCCommitted_def, metis)
+  next
+    case (TM_Abort x12a)
+    then show ?thesis using reach_trans
+      apply (auto simp add: tps_trans_defs tm_unchanged_defs tid_match_def TCCommitted_def)
+      by (metis status_tm.distinct(11))
+  next
+    case (TM_ReadyC x13a)
+    then show ?thesis using reach_trans
+      apply (auto simp add: tps_trans_defs tm_unchanged_defs tid_match_def TCCommitted_def)
+      by (metis status_tm.distinct(3))
+  next
+    case (TM_ReadyA x14)
+    then show ?thesis using reach_trans
+      apply (auto simp add: tps_trans_defs tm_unchanged_defs tid_match_def TCCommitted_def)
+      by (metis status_tm.distinct(3))
+  qed simp
+qed
+
+definition TCAborted where
+  "TCAborted s \<longleftrightarrow> (\<forall>cl. tm_status (tm s cl) = tm_aborted \<longrightarrow> 
+    (\<forall>k. tid_match s (get_txn_cl cl s) \<and>
+     km_status (kms s k) (get_txn_cl cl s) \<in> {read_lock, write_lock, no_lock, notokay, aborted}))"
+
+lemmas TCAbortedI = TCAborted_def[THEN iffD2, rule_format]
+lemmas TCAbortedE[elim] = TCAborted_def[THEN iffD1, elim_format, rule_format]
+
+lemma reach_tcaborted [simp, intro]: "reach tps s \<Longrightarrow> TCAborted s"
+proof(induction s rule: reach.induct)
+  case (reach_init s)
+  then show ?case
+  by (auto simp add: TCAborted_def tps_defs)
+next
+  case (reach_trans s e s')
+  then show ?case 
+  proof (cases e)
+    case (Write2 x11 x12 x13)
+    then show ?thesis using reach_trans
+      by (auto simp add: tps_trans_defs km_unchanged_defs tid_match_def TCAborted_def, smt)
+  next
+    case (Read2 x21 x22 x23)
+    then show ?thesis using reach_trans
+      by (auto simp add: tps_trans_defs km_unchanged_defs tid_match_def TCAborted_def, smt)
+  next
+    case (Prepare x31 x32)
+    then show ?thesis using reach_trans
+      apply (auto simp add: tps_trans_defs km_unchanged_defs tid_match_def TCAborted_def)
+      by (smt get_cl_txn.simps status_tm.distinct(9))
+  next
+    case (RLock x41 x42)
+    then show ?thesis using reach_trans
+      by (auto simp add: tps_trans_defs km_unchanged_defs tid_match_def TCAborted_def, smt)
+  next
+    case (WLock x51 x52)
+    then show ?thesis using reach_trans
+      by (auto simp add: tps_trans_defs km_unchanged_defs tid_match_def TCAborted_def, smt)
+  next
+    case (NoLock x61 x62)
+    then show ?thesis using reach_trans
+      by (auto simp add: tps_trans_defs km_unchanged_defs tid_match_def TCAborted_def, smt)
+  next
+    case (NOK x71 x72)
+    then show ?thesis using reach_trans
+      apply (auto simp add: tps_trans_defs km_unchanged_defs tid_match_def TCAborted_def)
+      by (smt get_cl_txn.simps status_tm.distinct(9))+
+  next
+    case (Commit x81 x82)
+    then show ?thesis using reach_trans
+      apply (auto simp add: tps_trans_defs km_unchanged_defs tid_match_def TCAborted_def)
+      by (smt get_cl_txn.simps status_tm.distinct(11))+
+  next
+    case (Abort x91 x92)
+    then show ?thesis using reach_trans
+      by (auto simp add: tps_trans_defs km_unchanged_defs tid_match_def TCAborted_def, smt+)
+  next
+    case (User_Commit x10)
+    then show ?thesis using reach_trans
+      apply (auto simp add: tps_trans_defs tm_unchanged_defs tid_match_def TCAborted_def)
+      by (smt status_tm.distinct(9))
+  next
+    case (TM_Commit x111 x112 x113 x114)
+    then show ?thesis using reach_trans
+      by (auto simp add: tps_trans_defs tm_unchanged_defs tid_match_def TCAborted_def, metis)
+  next
+    case (TM_Abort x12a)
+    then show ?thesis using reach_trans
+      by (auto simp add: tps_trans_defs tm_unchanged_defs tid_match_def TCAborted_def, metis)
+  next
+    case (TM_ReadyC x13a)
+    then show ?thesis using reach_trans
+      apply (auto simp add: tps_trans_defs tm_unchanged_defs tid_match_def TCAborted_def)
+      by (smt status_tm.distinct(5))
+  next
+    case (TM_ReadyA x14)
+    then show ?thesis using reach_trans
+      apply (auto simp add: tps_trans_defs tm_unchanged_defs tid_match_def TCAborted_def)
+      by (smt status_tm.distinct(5))
+  qed simp
+qed
+
+text\<open>Invariants about Shadow DB being empty after a commit and an abort\<close>
+definition TCCommitEmpF where
+  "TCCommitEmpF s \<longleftrightarrow> (\<forall>cl k. tm_status (tm s cl) = tm_committed
+      \<and> km_status (kms s k) (get_txn_cl cl s) = committed
+    \<longrightarrow> km_key_fp (kms s k) (get_txn_cl cl s) = Map.empty)"
+
+lemmas TCCommitEmpFI = TCCommitEmpF_def[THEN iffD2, rule_format]
+lemmas TCCommitEmpFE[elim] = TCCommitEmpF_def[THEN iffD1, elim_format, rule_format]
+
+lemma reach_tccommitempshadow [simp, intro]: "reach tps s \<Longrightarrow> TCCommitEmpF s"
+proof(induction s rule: reach.induct)
+  case (reach_init s)
+  then show ?case
+  by (auto simp add: TCCommitEmpF_def tps_defs)
+next
+  case (reach_trans s e s')
+  then show ?case 
+  proof (cases e)
+    case (Write2 x11 x12 x13)
+    then show ?thesis using reach_trans
+      apply (auto simp add: tps_trans_defs km_unchanged_defs TCCommitEmpF_def)
+      by (metis status_km.distinct(11))
+  next
+    case (Read2 x2)
+    then show ?thesis using reach_trans
+      apply (auto simp add: tps_trans_defs km_unchanged_defs TCCommitEmpF_def)
+      by (metis status_km.distinct(11))
+  next
+    case (Commit kc)
+    then show ?thesis using reach_trans
+      by (auto simp add: tps_trans_defs km_unchanged_defs TCCommitEmpF_def, metis+)
+  qed (auto simp add: tps_trans_defs intro!: TCCommitEmpFI)
+qed
+
+definition TCAbortEmpShadow where
+  "TCAbortEmpShadow s \<longleftrightarrow> (\<forall>k. tm_status (tm s) = tm_aborted \<and>
+                     ((km_status (kms s k) = working \<and> k_tid (kms s k) = Suc (tm_tid (tm s)))
+                      \<or> km_status (kms s k) = aborted)
+                  \<longrightarrow> k_shadow_db (kms s k) = empty_db)"
+
+lemmas TCAbortEmpShadowI = TCAbortEmpShadow_def[THEN iffD2, rule_format]
+lemmas TCAbortEmpShadowE[elim] = TCAbortEmpShadow_def[THEN iffD1, elim_format, rule_format]
+
+lemma reach_tcabortempshadow [simp, intro]: "reach tps s \<Longrightarrow> TCAbortEmpShadow s"
+proof(induction s rule: reach.induct)
+  case (reach_init s)
+  then show ?case
+  by (auto simp add: TCAbortEmpShadow_def tps_defs)
+next
+  case (reach_trans s e s')
+  then show ?case 
+  proof (cases e)
+    case (Write2 x11 x12 x13)
+    then show ?thesis using reach_trans
+      apply (auto simp add: tps_trans_defs other_insts_unchanged_def)
+      by (metis TCAbortEmpShadow_def n_not_Suc_n status_k.distinct(9))
+  next
+    case (Read2 x2)
+    then show ?thesis using reach_trans
+       apply (auto simp add: tps_trans_defs other_insts_unchanged_def)
+      by (metis TCAbortEmpShadow_def status_k.distinct(9))
+  next
+    case (Abort2 x7)
+    then show ?thesis using reach_trans
+      by (auto simp add: tps_trans_defs TCAbortEmpShadow_def other_insts_unchanged_def)
+  next
+    case (Ready x8)
+    then show ?thesis using reach_trans
+      by (auto simp add: tps_trans_defs TCAbortEmpShadow_def other_insts_unchanged_def)
+         metis+
+  next
+    case TM_Abort
+    then show ?thesis using reach_trans
+      apply(auto simp add: tps_trans_defs TCAbortEmpShadow_def other_insts_unchanged_def
+            dest!: reach_tcprepared)
+      by (metis status_k.distinct(31) status_k.distinct(39))
+  qed (auto simp add: tps_trans_defs intro!: TCAbortEmpShadowI)
+qed
+
+text\<open>Invariants about TID\<close>
+definition TCCommittedTID where
+  "TCCommittedTID s \<longleftrightarrow> (\<forall>k. tm_status (tm s) = tm_committed \<and> km_status (kms s k) = working
+                              \<longrightarrow> k_tid (kms s k) = Suc (tm_tid (tm s)))"
+
+lemmas TCCommittedTIDI = TCCommittedTID_def[THEN iffD2, rule_format]
+lemmas TCCommittedTIDE[elim] = TCCommittedTID_def[THEN iffD1, elim_format, rule_format]
+
+lemma reach_tccommittedtid [simp, intro]: "reach tps s \<Longrightarrow> TCCommittedTID s"
+proof(induction s rule: reach.induct)
+  case (reach_init s)
+  then show ?case
+  by (auto simp add: TCCommittedTID_def tps_defs)
+next
+  case (reach_trans s e s')
+  then show ?case 
+  proof (cases e)
+    case (Commit2 k)
+    then show ?thesis using reach_trans
+      apply (auto simp add: tps_trans_defs other_insts_unchanged_def intro!: TCCommittedTIDI)
+      by (metis TCCommittedTID_def status_k.distinct(7))
+  next
+    case (Ready k)
+    then show ?thesis using reach_trans
+      apply (auto simp add: tps_trans_defs other_insts_unchanged_def intro!: TCCommittedTIDI)
+      by (metis TCCommitted_def reach_tccommitted status_k.distinct(3) status_k.distinct(7))
+  qed (auto simp add: tps_trans_defs intro!: TCCommittedTIDI)
+qed
+
+definition TCAbortedTID where
+  "TCAbortedTID s \<longleftrightarrow> (\<forall>k. tm_status (tm s) = tm_aborted \<and> km_status (kms s k) = working
+                            \<longrightarrow> k_tid (kms s k) = Suc (tm_tid (tm s)))"
+
+lemmas TCAbortedTIDI = TCAbortedTID_def[THEN iffD2, rule_format]
+lemmas TCAbortedTIDE[elim] = TCAbortedTID_def[THEN iffD1, elim_format, rule_format]
+
+lemma reach_tcabortedtid [simp, intro]: "reach tps s \<Longrightarrow> TCAbortedTID s"
+proof(induction s rule: reach.induct)
+  case (reach_init s)
+  then show ?case
+  by (auto simp add: TCAbortedTID_def tps_defs)
+next
+  case (reach_trans s e s')
+  then show ?case 
+  proof (cases e)
+    case (Abort2 x7)
+    then show ?thesis using reach_trans
+      apply (auto simp add: tps_trans_defs other_insts_unchanged_def intro!: TCAbortedTIDI)
+      by (metis TCAbortedTID_def status_k.distinct(9))+
+  next
+    case (Ready x9)
+    then show ?thesis using reach_trans
+      apply (auto simp add: tps_trans_defs other_insts_unchanged_def intro!: TCAbortedTIDI)
+      by (metis TCAbortedTID_def TCAborted_def reach_tcaborted status_k.distinct(9))
+  next
+    case TM_Abort
+    then show ?thesis using reach_trans
+      apply (auto simp add: tps_trans_defs other_insts_unchanged_def intro!: TCAbortedTIDI)
+      by (metis status_k.distinct(3) status_k.distinct(5))
+  qed (auto simp add: tps_trans_defs intro!: TCAbortedTIDI)
+qed
+
+subsection \<open>Refinement from ET_ES to tps\<close>
+
+subsubsection \<open>Mediator function\<close>
+
+fun med :: "'v ev \<Rightarrow> 'v label" where
+  "med (TM_ev cl (TM_Commit sn u F)) = (ET cl sn u F)" |
+  "med _ = Skip"
+
+
+subsubsection \<open>Simulation function\<close>
+
+lemma write_lock_inv: "\<forall>t. km_status (kms gs k) t \<noteq> write_lock \<or> (\<exists>! t. km_status (kms gs k) t = write_lock)"
+proof (cases "km_status (kms gs k) t")
+  case working
+  then show ?thesis sorry
+next
+  case prepared
+  then show ?thesis sorry
+next
+  case read_lock
+  then show ?thesis sorry
+next
+case write_lock
+  then show ?thesis sorry
+next
+  case no_lock
+  then show ?thesis sorry
+next
+  case notokay
+  then show ?thesis sorry
+next
+  case committed
+  then show ?thesis sorry
+next
+  case aborted
+then show ?thesis sorry
+qed
+
+fun update_kv_reads_all_txn :: "(txid0 \<Rightarrow> 'v key_fp) \<Rightarrow> key_view \<Rightarrow> 'v v_list \<Rightarrow> 'v v_list" where
+  "update_kv_reads_all_txn tFk uk vl =
+    (let lv = last_version vl uk in
+      vl[Max uk := lv\<lparr>v_readerset := (v_readerset lv) \<union> {t.\<exists>v. tFk t R = Some v}\<rparr>])"
+
+fun kvs_of_gs :: "'v global_state \<Rightarrow> 'v kv_store" where
+  "kvs_of_gs gs k =
+    (if tm_status (tm gs cl) = tm_committed then
+        update_kv_reads_all_txn (\<lambda>t. km_key_fp (kms gs k) t) uk (km_vl (kms gs k))
+     else 
+        km_vl (kms gs k)
+    )"
+
+fun last_touched_version :: "txid0 \<Rightarrow> 'v v_list \<Rightarrow> v_id" where
+  "last_touched_version t [] = 0" |
+  "last_touched_version t (x # rest) =
+    (if Tn t = v_writer x \<or> t \<in> v_readerset x then length rest else last_touched_version t rest)"
+
+definition cl_last_view :: "cl_id \<Rightarrow> sqn \<Rightarrow> 'v kv_store \<Rightarrow> view" where
+  "cl_last_view cl sn K k \<equiv> {..<(last_touched_version (Tn_cl sn cl) (rev (K k)))}"
+
+fun views_of_gs :: "'v global_state \<Rightarrow> (cl_id \<Rightarrow> view)" where
+  "views_of_gs gs = (\<lambda>cl.
+    (if tm_status (tm gs cl) = tm_committed then
+       (\<lambda>k. full_view (kvs_of_gs gs k))
+     else cl_last_view cl (tm_sn (tm gs cl)) (\<lambda>k. km_vl (kms gs k)))
+    )"
+
+definition sim :: "'v global_state \<Rightarrow> 'v config" where
+  "sim gs = (kvs_of_gs gs, views_of_gs gs)"
+
+
+lemma union_db_write:
+  assumes
+    "k_shadow_db (kms gs' (loc k)) = db_write (k_shadow_db (kms gs (loc k))) k v"
+    "other_insts_unchanged (loc k) (kms gs) (kms gs')"
+  shows
+    "union_db (\<lambda>k. k_shadow_db (kms gs' k)) = db_write (union_db (\<lambda>k. k_shadow_db (kms gs k))) k v"
+  using assms
+  apply (auto simp add: union_db_def)
+  apply (rule ext)
+  subgoal for k'
+    by (cases "loc k = loc k'") (auto simp add: db_write_def other_insts_unchanged_def)
+  done
+
+lemma tps_refines_tps1: "tps \<sqsubseteq>\<^sub>\<pi>21 tps1"
+proof (intro simulate_ES_fun_with_invariant[where I="\<lambda>s. TCCommittedTID s \<and> TCCommitEmpF s \<and> TCAbortedTID s \<and> TCAbortEmpShadow s"])
+  fix gs0
+  assume p: "init tps gs0"
+  then show "init tps1 (sim21 gs0)" using p
+    by (auto simp add: tps1_defs tps_defs union_db_def)
+next
+  fix gs a gs'
+  assume p: "tps: gs\<midarrow>a\<rightarrow> gs'"
+     and inv: "TCCommittedTID gs \<and> TCCommitEmpF gs \<and> TCAbortedTID gs \<and> TCAbortEmpShadow gs"
+  then show "tps1: sim21 gs\<midarrow>\<pi>21 a\<rightarrow> sim21 gs'"
+  proof (cases a)
+    case (Write2 k k v)
+    then show ?thesis using p inv
+      apply (auto simp add: tps_trans_defs tps1_trans_defs union_db_write)
+      by (metis other_insts_unchanged_def)
+  next
+    case (Read2 k k ov)
+    then show ?thesis using p inv
+      apply (auto simp add: tps_trans_defs tps1_trans_defs)
+      apply (metis other_insts_unchanged_def)
+      apply (metis other_insts_unchanged_def)
+      by (simp add: map_add_def union_db_def)
+  next
+    case (Prepare k)
+    then show ?thesis using p
+      apply (auto simp add: tps_trans_defs tps1_trans_defs)
+      by (metis other_insts_unchanged_def)+
+  next
+    case (OK x4)
+    then show ?thesis using p
+      apply (auto simp add: tps_trans_defs tps1_trans_defs)
+      by (metis other_insts_unchanged_def)+
+  next
+    case (NOK x5)
+    then show ?thesis using p
+      apply (auto simp add: tps_trans_defs tps1_trans_defs)
+      by (metis other_insts_unchanged_def)+
+  next
+    case (PrepUAbort x6)
+    then show ?thesis using p
+      apply (auto simp add: tps_trans_defs tps1_trans_defs)
+      by (metis other_insts_unchanged_def)+
+  next
+    case (UAbort2 k)
+    then show ?thesis using p
+      apply (auto simp add: tps_trans_defs tps1_trans_defs)
+      apply (metis other_insts_unchanged_def)
+      by (metis other_insts_unchanged_def)
+  next
+    case (Commit2 k)
+    then show ?thesis using p inv
+      apply (auto simp add: tps_trans_defs tps1_trans_defs)
+      by (smt commit2_def gs_trans.simps(6) map_add_empty
+          other_insts_unchanged_def p tps_trans union_db_eq_cases)
+  next
+    case (Abort2 k)
+    then show ?thesis using p
+      apply (auto simp add: tps_trans_defs tps1_trans_defs)
+      by (metis other_insts_unchanged_def)+
+  next
+    case (Ready k)
+    then show ?thesis using p inv
+      apply (auto simp add: tps_trans_defs tps1_trans_defs)
+      apply (smt other_insts_unchanged_def union_db_eq_cases)
+      by (metis other_insts_unchanged_def)
+  next
+    case TM_Commit
+    then show ?thesis using p
+      by (auto simp add: tps_trans_defs tps1_trans_defs map_add_union_db)
+  next
+    case TM_ReadyC
+    then show ?thesis using p inv
+      by (auto simp add: tps_trans_defs tps1_trans_defs union_db_def)
+  next
+    case TM_ReadyA
+    then show ?thesis using p inv
+      by (auto simp add: tps_trans_defs tps1_trans_defs union_db_def)
+  qed (auto simp add: tps_trans_defs tps1_trans_defs)
+qed auto
 
 
 end
